@prefix : <urn:webprotege:ontology:c5284879-633c-4b00-8fb5-29d44036ba9b#> .
@prefix owl: <http://www.w3.org/2002/07/owl#> .
@prefix rdf: <http://www.w3.org/1999/02/22-rdf-syntax-ns#> .
@prefix xml: <http://www.w3.org/XML/1998/namespace> .
@prefix xsd: <http://www.w3.org/2001/XMLSchema#> .
@prefix frbr: <http://iflastandards.info/ns/fr/frbr/frbroo/> .
@prefix lime: <http://www.w3.org/ns/lemon/lime#> .
@prefix rdfs: <http://www.w3.org/2000/01/rdf-schema#> .
@prefix lexicog: <http://www.w3.org/ns/lemon/lexicog#> .
@prefix ontolex: <http://www.w3.org/ns/lemon/ontolex#> .
@base <urn:absolute:lexicographic_resource_ontology> .

<urn:absolute:lexicographic_resource_ontology> rdf:type owl:Ontology ;
                                                owl:imports <http://www.w3.org/ns/lemon/lexicog> ;
                                                <http://purl.org/dc/elements/1.1/creator> "Fahad Khan"@en ;
                                                rdfs:comment "An ontology for representing lexicographic resources using pre-existing vocabularies."@en .

#################################################################
#    Object Properties
#################################################################

###  http://purl.org/spar/cito/citesAsEvidence
<http://purl.org/spar/cito/citesAsEvidence> rdf:type owl:ObjectProperty .


###  urn:webprotege:ontology:c5284879-633c-4b00-8fb5-29d44036ba9b#citesAsAttestation
:citesAsAttestation rdf:type owl:ObjectProperty ;
                    rdfs:subPropertyOf <http://purl.org/spar/cito/citesAsEvidence> ;
                    rdfs:comment "A subproperty of the CiTO property citesAsEvidence where the citing entity cites the cited entity as attesting to the existence of a linguistic phenomenon or phenomena."@en .


#################################################################
#    Classes
#################################################################

###  http://iflastandards.info/ns/fr/frbr/frbroo/F1_Expression
frbr:F1_Expression rdf:type owl:Class .


###  http://iflastandards.info/ns/fr/frbr/frbroo/F1_Work
frbr:F1_Work rdf:type owl:Class .


###  http://www.w3.org/ns/lemon/lime#Lexicon
lime:Lexicon rdf:type owl:Class .


###  urn:webprotege:ontology:c5284879-633c-4b00-8fb5-29d44036ba9b#LexicographicExpression
:LexicographicExpression rdf:type owl:Class ;
                         rdfs:subClassOf frbr:F1_Expression ,
                                         lexicog:LexicographicResource ;
                         rdfs:comment "Comprises an intellectual realisation of the description of a lexicon as a structured text."@en ;
                         rdfs:label "Lexicographic Expression"@en .


###  urn:webprotege:ontology:c5284879-633c-4b00-8fb5-29d44036ba9b#LexicographicWork
:LexicographicWork rdf:type owl:Class ;
                   rdfs:subClassOf frbr:F1_Work ,
                                   lime:Lexicon ;
                   rdfs:comment "Comprises concepts or combinations of concepts for representing/describing the lexicon for a given language community or communities or domain."@en ;
                   rdfs:label "Lexicographic Work"@en .


###  Generated by the OWL API (version 4.5.9.2019-02-01T07:24:44Z) https://github.com/owlcs/owlapi
